rocq/theories/TypeSystem/CheckerUsageSoundness.v
@@ -107,6 +107,7 @@ Fixpoint expr_linear_lets_used (fenv : list fn_def) (e : expr) {struct e}
   | ELit _ => True
   | EVar _ => True
   | EFn _ => True
+  | EMakeClosure _ _ => True
   | EPlace _ => True
   | ELet m x T e1 e2 =>
       (ty_usage T = ULinear ->
